# Chapter 4: Algebra

---
In this chapter, I've learned:

### **Ex.33**

---
Consider all properties of a communicative group on $Z_5^*$, we have:  

- **Commutativity**: for all elements $g_1$, $g_2 \in Z_5^*$, we have $g_1\cdot g_2 = g_2\cdot g_1$.  
- **Associativity**: for all elements  $g_1$, $g_2$, $g_3 \in Z_5^*$, we have
$g_1\cdot (g_2\cdot g_3) =(g_1\cdot g_2)\cdot g_3$.  
- **Existence of a neutral element**: $1$ is the neutral element of $Z_5^*$.  
- **Existence of an inverse**: all elements in $Z_5^*$ have inverse.  
So that $Z_5^*$ is a communicative group.  

### **Ex.34**

---
With $n$ is a prime number, $(Z_n^*, \cdot)$ is a communicative group with $1$ is the neutral element.

### **Ex.35**

---
The remainder class will have element from $0$ to $n-1$, so the order of $(Z_n, +)$ is $n$.

### **Ex.36**

---
We have $5^1=5$, $5^2=4$, $5^3=3$, $5^4=2$, $5^5=1$, $5^6=0$. We can generate all elements of $Z_6^*$ by multiply $5$,
so that $5$ is a generator.  
Do the same to $2$, we will have the result that can't generate all elements of $Z_6^*$ by multiply $2$, so $2$ is not
a generator.

### **Ex.37**

---

### **Ex.38**

### **Ex.39**

---
Consider all properties of a communicative group on $Z_5^*[2]$, we have:

- Commutativity: Same as $Z_5^*$.
- Associativity: Same as $Z_5^*$.
- Existence of a neutral element: 1 is the neutral element of $Z_5^*[2]$.
- Existence if an inverse: since $4\cdot 4=1$ and $1\cdot 1=1$ over $Z_5^*[2]$, all elements in $Z_5^*[2]$ have inverse.
So that $Z_5^*[2]$ is a communicative group.

### **Ex.40**

---
Since $6=3\cdot2\cdot1$, we have all subgroup of $Z_6$ as below:  

- $Z_6[1]=\{0\}$
- $Z_6[2]=\{0, 2\}$
- $Z_6[3]=\{0,2,4\}$
- $Z_6[6]=\{0,1,3,2,4,5\}$
$3$ is the large prime order subgroup of $Z_6$, we get the cofactor clearing map $(+)^2: Z_6\rightarrow Z_6[3]$:  
- $0+0=0,$
- $1+1=2,$
- $2+2=4,$
- $3+3=0,$
- $4+4=2,$
- $5+5=4$

### **Ex.41**

---

### **Ex.42**

---
For $G_1$ we have $g_1, g_1' \in G_1$, for $G_2$ we have $g_2, g_2' \in G_2$.
If $g_1=g_1'$ we have $e(g_1^a, g_2)=e(g_1,g_2)\cdot e(g_1,g_2)\cdot ...=e(g_1,g_2)^a$.  
If $g_2=g_2'$ we have $e(g_1^a, g_2^b)=e(g_1^a,g_2)\cdot e(g_1^a,g_2)\cdot ...=e(g_1,g_2)^{a\cdot b}$.  

### **Ex.43**

---
